src/Dafny/machine/machine.model.dfy
@@ -1,10 +1,20 @@
-include "machine_s.dfy"
+include "machine.s.dfy"
+
+// This model ensures that the bytes extern interface is feasible (that it has
+// no contradictions). See
+// https://github.com/dafny-lang/dafny/wiki/Modeling-External-State-Correctly
+// for a complete description of this approach.
 
 module bytes_model refines bytes {
     class {:compile false} Bytes {
         var data_: seq<byte>;
 
-        function data(): seq<byte>
+        predicate Valid()
+        {
+            |data_| < 0x1_0000_0000_0000_0000
+        }
+
+        function method data(): seq<byte>
         {
             data_
         }
@@ -14,10 +24,9 @@ module bytes_model refines bytes {
             this.data_ := data_;
         }
 
-        method Get(i: uint64)
-        returns (x:byte)
+        function method Get(i: uint64): (x:byte)
         {
-            return data_[i];
+            data_[i]
         }
 
         method Append(b: byte)
@@ -27,7 +36,8 @@ module bytes_model refines bytes {
     }
 
     method {:compile false} NewBytes(sz: uint64)
-    returns (bs:Bytes) {
-        return new Bytes(repeat(0 as byte, sz as nat));
+    returns (bs:Bytes)
+    {
+       return new Bytes(repeat(0 as byte, sz as nat));
     }
 }
