src/Dafny/machine/int_encoding.s.dfy
@@ -4,12 +4,13 @@ Experiment with little-endian encoding of integers.
 IronFleet has good code for this at
 https://github.com/GLaDOS-Michigan/IronFleet/blob/master/ironfleet/src/Dafny/Distributed/Impl/Common/Util.i.dfy
 */
-include "machine_s.dfy"
+include "machine.s.dfy"
 
 module IntEncoding
 {
 
 import opened Machine
+import opened bytes
 
 function le_enc16(x: bv16): (bs:seq<byte>)
 ensures |bs| == 2
@@ -40,5 +41,28 @@ function method {:axiom} le_dec64(bs: seq<byte>): uint64
 requires |bs| == 8
 lemma {:axiom} lemma_le_enc_dec64(x: uint64)
 ensures le_dec64(le_enc64(x)) == x
+
+lemma split_at_last<T>(xs: seq<T>, k: nat)
+requires 1 <= k < |xs|
+ensures xs[..k] == xs[..k-1] + [xs[k-1]]
+{}
+
+lemma singleton_eq<T>(x1: T, x2: T)
+requires x1 == x2
+ensures [x1] == [x2]
+{}
+
+method {:extern} UInt64Put(x: uint64, off: uint64, bytes: Bytes)
+modifies bytes
+requires bytes.Valid() ensures bytes.Valid()
+requires off as nat + 8 <= |bytes.data()|
+ensures bytes.data() == old(bytes.data()[..off as nat] + le_enc64(x) + bytes.data()[off as nat+8..])
+
+method {:extern} UInt64Get(bytes: Bytes, off: uint64)
+returns (x:uint64)
+requires bytes.Valid()
+requires off as nat + 8 <= |bytes.data()|
+ensures x == le_dec64(bytes.data()[off as nat..off as nat+8])
+
 
 }
