Makefile
@@ -1,4 +1,4 @@
-DFY_FILES := $(shell find src -path src/Dafny/machine/machine_s-go -prune -false -o -name "*.dfy")
+DFY_FILES := $(shell find src -path src/Dafny/machine/machine.s-go -prune -false -o -name "*.dfy")
 OK_FILES := $(DFY_FILES:.dfy=.dfy.ok)
 
 DAFNY_ARGS := /compile:0 /compileTarget:go /nologo /compileVerbose:0
@@ -6,7 +6,7 @@ DAFNY := ./etc/dafnyq $(DAFNY_ARGS)
 
 Q:=@
 
-all: $(OK_FILES) src/Dafny/machine/machine_s-go/src/machine_s.go
+all: $(OK_FILES) src/Dafny/machine/machine.s-go/src/machine.s.go
 
 .dafnydeps.d: $(DFY_FILES) etc/dafnydep
 	@echo "DAFNYDEP"
@@ -22,7 +22,7 @@ endif
 	$(Q)$(DAFNY) /compile:0 "$<" 1>/dev/null
 	$(Q)touch "$@"
 
-src/Dafny/machine/machine_s-go/src/machine_s.go: src/Dafny/machine/machine_s.dfy
+src/Dafny/machine/machine.s-go/src/machine.s.go: src/Dafny/machine/machine.s.dfy
 	@echo "DAFNY COMPILE $<"
 	$(Q)$(DAFNY) /countVerificationErrors:0 /spillTargetCode:2 $< 1>/dev/null
 
@@ -30,4 +30,4 @@ clean:
 	@echo "CLEAN"
 	$(Q)find . -name "*.dfy.ok" -delete
 	$(Q)rm -f .dafnydeps.d
-	$(Q)rm -rf src/Dafny/machine/machine_s-go
+	$(Q)rm -rf src/Dafny/machine/machine.s-go
